\documentclass[10pt,a4paper, margin=1in]{article}
\usepackage{fullpage}
\usepackage{amsfonts, amsmath, pifont}
\usepackage{amsthm}
\usepackage{graphicx}
\usepackage{float}

\usepackage{tkz-euclide}
\usepackage{tikz}
\usepackage{pgfplots}
\pgfplotsset{compat=1.13}

\usepackage{geometry}
 \geometry{
 a4paper,
 total={210mm,297mm},
 left=10mm,
 right=10mm,
 top=10mm,
 bottom=10mm,
 }
 % Write both of your names here. Fill exxxxxxx with your ceng mail address.
 \author{
  Geçit, Emre\\
  \texttt{e2521581@ceng.metu.edu.tr}
  \and
  Yancı, Baran\\
  \texttt{e2449015@ceng.metu.edu.tr}
}

\title{CENG 384 - Signals and Systems for Computer Engineers \\
Spring 2023 \\
Homework 2}
\begin{document}
\maketitle



\noindent\rule{19cm}{1.2pt}

\begin{enumerate}

\item %write the solution of q1
    \begin{enumerate}
    % Write your solutions in the following items.
    \item %write the solution of q1a
    \begin{align*}
        y(t) & = x(t) - 5 \dot{y}(t) \\
    \end{align*}
    \item %write the solution of q1b
    \begin{align*}
        y(t) & = (e^{-t} + e^{-3t})u(t) - 5 \dot{y}(t) \\
        y(t) + 5 \dot{y}(t) & = (e^{-t} + e^{-3t})u(t) \\
        y(t) & = y_p(t) + y_h(t) \\
        y_p(t) & = Ke^{-t}u(t) + Le^{-3t}u(t) \\
        Ke^{-t}u(t) + Le^{-3t}u(t) + 5 (-Ke^{-t}u(t) -3Le^{-3t}u(t)) & = (e^{-t} + e^{-3t})u(t) \\
        Ke^{-t}u(t) + Le^{-3t}u(t) - 5Ke^{-t}u(t) - 15Le^{-3t}u(t) & = (e^{-t} + e^{-3t})u(t) \\
        e^{-t}u(t) (K - 5K) + e^{-3t}u(t) (L - 15L) & = (e^{-t} + e^{-3t})u(t) \\
        K - 5K & = 1 \\
        K & = - 1/4 \\
        L - 15L & = 1 \\
        L & = - 1/14 \\
        y_p(t) & = \frac{-1}{4}e^{-t}u(t) + \frac{-1}{14}e^{-3t}u(t) \\
        y_h(t) & = c_1e^{\alpha t} \\
        c_1e^{\alpha t} + 5\alpha c_1e^{\alpha t} & = 0 \\
        c_1 + 5\alpha c_1 & = 0 \\
        \alpha & = \frac{-1}{5} \\
        y_h(t) & = c_1e^{\frac{-1}{5}t} \\
        y(t) & = y_p(t) + y_h(t) \\
        & = \frac{-1}{4}e^{-t}u(t) + \frac{-1}{14}e^{-3t}u(t) + c_1e^{\frac{-1}{5}t} \\
        y(0) & = 0 \\
        0 & = \frac{-1}{4} + \frac{-1}{14} + c_1 \\
        c_1 & = \frac{9}{28} \\
        y(t) & = \frac{-1}{4}e^{-t}u(t) + \frac{-1}{14}e^{-3t}u(t) + \frac{9}{28}e^{\frac{-1}{5}t} \\
    \end{align*}
    \end{enumerate}

\item %write the solution of q2  
	\begin{enumerate}
    % Write your solutions in the following items.
    \item %write the solution of q2a
    \begin{align*}
        y[n] & = x[n] * h[n] \\
        & = \sum_{k=0}^{n} x[k]h[n-k] \\
        & = \sum_{k=0}^{n} \left(2\delta [k] + \delta [k + 1]\right) \left(\delta [n-(1+k)] + 2\delta [n+1-k]\right) \\
        & = 2\sum_{k=0}^{n} \delta [k] \delta [n-(1+k)] + 4\sum_{k=0}^{n} \delta [k] \delta [n+1-k] + \sum_{k=0}^{n} \delta [k + 1] \delta [n-(1+k)] + 2\sum_{k=0}^{n} \delta [k + 1] \delta [n+1-k] \\
        & = 2\delta\left[\frac{n-1}{2}\right] + 4\delta\left[\frac{n+1}{2}\right] + \delta\left[\frac{n-2}{2}\right] + 2\delta\left[\frac{n}{2}\right] \\
    \end{align*}

    % TODO: drawing

    \item %write the solution of q2b
    % TODO: this feels wrong
    \begin{align*}
        y(t) & = \frac{dx(t)}{dt} * h(t) \\
        & = \frac{d}{dt}\left(u(t-1) + u(t+1)\right) * e^{-t} \sin (t)u(t) \\
        & = \left(\delta(t-1) - \delta(t+1)\right) * e^{-t} \sin (t)u(t) \\
        & = \int_{-\infty}^{\infty} \left(\delta(\tau-1) - \delta(\tau+1)\right) e^{-t - \tau} \sin (t - \tau) d\tau \\
        & = \int_{-\infty}^{\infty} \delta(\tau-1)e^{-t - \tau} \sin (t - \tau) d\tau - \int_{-\infty}^{\infty} \delta(\tau+1) e^{-t - \tau} \sin (t - \tau) d\tau \\
        & = e^{-t - 1} \sin (t - 1)u(t) + e^{-t + 1} \sin (t + 1)u(t) \\
    \end{align*}
    \end{enumerate}

\item %write the solution of q3
    \begin{enumerate}
    % Write your solutions in the following items.
    \item %write the solution of q3a

    % @y4nci: see https://odtuclass2022s.metu.edu.tr/pluginfile.php/523917/mod_resource/content/14/week_4.html#convolution-operation-in-continuous-time exercise 4.1

    \begin{align*}
        y(t) & = x(t) * h(t) \\
        & = \int_{-\infty}^{\infty} x(\tau) h(t - \tau) d\tau \\
        & = \int_{-\infty}^{\infty} x(t - \tau) h(\tau) d\tau \\
        & = \int_{-\infty}^{\infty} e^{-(t - \tau)} e^{-2\tau} d\tau \\
        & = \int_{0}^{t} e^{-(t - \tau)} e^{-2\tau} d\tau \\
        & = e^{-t} \int_{0}^{t} e^{\tau} d\tau \\
        & = e^{-t} \left(1 - e^{-t}\right)u(t) \\
    \end{align*}
    \item %write the solution of q3b
    \begin{align*}
        y(t) & = x(t) * h(t) \\
        & = \int_{-\infty}^{\infty} x(\tau) h(t - \tau) d\tau \\
        & = \int_{-\infty}^{\infty} x(t - \tau) h(\tau) d\tau \\
        & = \int_{-\infty}^{\infty} \left(u(t - \tau) - u(t - (\tau + 1))\right) e^{3\tau} d\tau \\
        & = \int_{-\infty}^{\infty} u(t - \tau) e^{3\tau} d\tau - \int_{-\infty}^{\infty} u(t - (\tau + 1)) e^{3\tau} d\tau \\
        & = \int_{-\infty}^{t} e^{3\tau} d\tau - \int_{-\infty}^{t - 1} e^{3\tau} d\tau \\
        & = \frac{e^{3t}}{3} - \frac{e^{3t - 3}}{3}\\
    \end{align*}
    \end{enumerate}

\item %write the solution of q4
    \begin{enumerate}   
    % Write your solutions in the following items.
    \item %write the solution of q4a
    \item %write the solution of q4b
    \end{enumerate}

\item %write the solution of q5
    \begin{enumerate}
    % Write your solutions in the following items.
    \item %write the solution of q5a
    \item %write the solution of q5b
	\item %write the solution of q5c
    \end{enumerate}    
    
\item %write the solution of q6
    \begin{enumerate}
    % Write your solutions in the following items.
    \item %write the solution of q6a
    \item %write the solution of q6b
	\item %write the solution of q6c
    \end{enumerate}
    
\item %write the solution of q7
    \begin{enumerate}
    % Write your solutions in the following items.
    \item %write the solution of q7a
    \item %write the solution of q7b
    \end{enumerate}    

\end{enumerate}


\end{document}

