\documentclass[10pt,a4paper, margin=1in]{article}
\usepackage{fullpage}
\usepackage{amsfonts, amsmath, pifont}
\usepackage{amsthm}
\usepackage{graphicx}
\usepackage{float}

\usepackage{tkz-euclide}
\usepackage{tikz}
\usepackage{pgfplots}
\pgfplotsset{compat=1.13}

\usepackage{geometry}
 \geometry{
 a4paper,
 total={210mm,297mm},
 left=10mm,
 right=10mm,
 top=10mm,
 bottom=10mm,
 }
 \author{
  Geçit, Emre\\
  \texttt{e2521581@ceng.metu.edu.tr}
  \and
  Yancı, Baran\\
  \texttt{e2449015@ceng.metu.edu.tr}
}

\title{CENG 384 - Signals and Systems for Computer Engineers \\
Spring 2023 \\
Homework 4}
\begin{document}
\maketitle



\noindent\rule{19cm}{1.2pt}

\begin{enumerate}

\item %write the solution of q1
	\begin{enumerate}   
    % Write your solutions in the following items.
    \item %write the solution of q1a
    \begin{align*}
        H(j\omega) &= \frac{j\omega - 1}{j\omega + 1} \\
        \frac{Y(j\omega)}{X(j\omega)} &= \frac{j\omega - 1}{j\omega + 1} \\
        Y(j\omega)(j\omega + 1) &= X(j\omega)(j\omega - 1) \\
        y'(t) + y(t) &= x'(t) - x(t) \\
    \end{align*}
    \item %write the solution of q1b
    % find the impulse response
    \begin{align*}
        H(j\omega) &= \frac{j\omega - 1}{j\omega + 1} \\
        h(t) &= \mathcal{F}^{-1}\{H(j\omega)\} \\
        &= \mathcal{F}^{-1}\{\frac{j\omega - 1}{j\omega + 1}\} \\
        &= \mathcal{F}^{-1}\{\frac{j\omega + 1 - 2}{j\omega + 1}\} \\
        &= \mathcal{F}^{-1}\{\frac{j\omega + 1}{j\omega + 1}\} - \mathcal{F}^{-1}\{\frac{2}{j\omega + 1}\} \\
        &= \mathcal{F}^{-1}\{1\} - 2\mathcal{F}^{-1}\{\frac{1}{j\omega + 1}\} \\
        &= \delta(t) - 2e^{-t}u(t) \\
    \end{align*}
	\item %write the solution of q1c
    % find and plot the output for the input x(t) = e^{-2t}u(t)
    \begin{align*}
        y'(t) + y(t) &= x'(t) - x(t) \\
        y'(t) + y(t) &= -2e^{-2t}u(t) - e^{-2t}u(t) \\
        y'(t) + y(t) &= -3e^{-2t}u(t) \\
        y_p(t) &= Ae^{-2t} \\
        y_p'(t) &= -2Ae^{-2t} \\
        -2Ae^{-2t} + Ae^{-2t} &= -3e^{-2t}u(t) \\
        A &= 3 \\
        y_p(t) &= 3e^{-2t} \\
        y_h(t) &= c_1e^{-t}u(t) \\
        y(t) &= y_p(t) + y_h(t) \\
        &= 3e^{-2t} + c_1e^{-t}u(t) \\
        y(0) &= 0 \\
        0 &= 3e^{-2(0)} + c_1e^{-0}u(0) \\
        0 &= 3 + c_1 \\
        c_1 &= -3 \\
        y(t) &= 3e^{-2t} - 3e^{-t}u(t) \\
    \end{align*}
    \item %write the solution of q1d
    % TODO: draw
    \end{enumerate}

\item %write the solution of q2  
	\begin{enumerate}
    % Write your solutions in the following items.
    \item %write the solution of q2a
    \begin{align*}
        y[n + 1] - \frac{1}{2}y[n] &= x[n + 1] \\ 
        e^{j\omega}Y(e^{j\omega}) - \frac{1}{2}Y(e^{j\omega}) &= e^{j\omega}X(e^{j\omega}) \\
        H(e^{j\omega}) &= \frac{Y(e^{j\omega})}{X(e^{j\omega})} \\
        H(e^{j\omega}) &= \frac{e^{j\omega}}{e^{j\omega} - \frac{1}{2}} \\
    \end{align*}
    \item %write the solution of q2b
    % fiind the impulse response
    \begin{align*}
        H(e^{j\omega}) &= \frac{e^{j\omega}}{e^{j\omega} - \frac{1}{2}} \\
        h[n] &= \mathcal{F}^{-1}\{H(e^{j\omega})\} \\
        &= \mathcal{F}^{-1}\{\frac{e^{j\omega}}{e^{j\omega} - \frac{1}{2}}\} \\
        &= \mathcal{F}^{-1}\{\frac{e^{j\omega} - \frac{1}{2} + \frac{1}{2}}{e^{j\omega} - \frac{1}{2}}\} \\
        &= \mathcal{F}^{-1}\{\frac{e^{j\omega} - \frac{1}{2}}{e^{j\omega} - \frac{1}{2}} + \frac{\frac{1}{2}}{e^{j\omega} - \frac{1}{2}}\} \\
        &= \mathcal{F}^{-1}\{1 + \frac{\frac{1}{2}}{e^{j\omega} - \frac{1}{2}}\} \\
        &= \mathcal{F}^{-1}\{1\} + \mathcal{F}^{-1}\{\frac{\frac{1}{2}}{e^{j\omega} - \frac{1}{2}}\} \\
        &= \delta[n] + \frac{1}{2}\mathcal{F}^{-1}\{\frac{1}{e^{j\omega} - \frac{1}{2}}\} \\
        &= \delta[n] + \frac{1}{2}e^{\frac{1}{2}n}u[n] \\
    \end{align*}
	\item %write the solution of q2c
    % find and plot the output for the input x[n] = \left(\frac{3}{4}\right)^nu[n]
    \begin{align*}
        y[n + 1] - \frac{1}{2}y[n] &= x[n + 1] \\ 
        y[n + 1] - \frac{1}{2}y[n] &= \left(\frac{3}{4}\right)^{n + 1}u[n + 1] \\ 
        y_p[n] &= A\left(\frac{3}{4}\right)^n \\
        y_p[n + 1] &= A\left(\frac{3}{4}\right)^{n + 1} \\
        A\left(\frac{3}{4}\right)^{n + 1} - \frac{1}{2}A\left(\frac{3}{4}\right)^n &= \left(\frac{3}{4}\right)^{n + 1}u[n + 1] \\
        \frac{3}{4}A\left(\frac{3}{4}\right)^n - \frac{1}{2}A\left(\frac{3}{4}\right)^n &= \frac{3}{4}\left(\frac{3}{4}\right)^nu[n + 1] \\
        \frac{3}{4}A - \frac{1}{2}A &= \frac{3}{4}u[n + 1] \\
        A &= 3 \\
        y_p[n] &= 3\left(\frac{3}{4}\right)^n \\
        y_h[n] &= c_1\left(\frac{1}{2}\right)^nu[n] \\
        y[n] &= y_p[n] + y_h[n] \\
        &= 3\left(\frac{3}{4}\right)^n + c_1\left(\frac{1}{2}\right)^nu[n] \\
        y[0] &= 0 \\
        0 &= 3\left(\frac{3}{4}\right)^0 + c_1\left(\frac{1}{2}\right)^0u[0] \\
        0 &= 3 + c_1 \\
        c_1 &= -3 \\
        y[n] &= 3\left(\frac{3}{4}\right)^n - 3\left(\frac{1}{2}\right)^nu[n] \\
    \end{align*}
    \end{enumerate}

\item %write the solution of q3
	\begin{enumerate}
    % Write your solutions in the following items.
    \item %write the solution of q3a
    \begin{align*}
        H(j\omega) &= H_1(j\omega)H_2(j\omega) \\
        &= \frac{1}{j\omega + 1}\frac{1}{j\omega + 2} \\
        &= \frac{Y(j\omega)}{X(j\omega)} \\
        Y(j\omega)(j\omega + 1)(j\omega + 2) &= X(j\omega) \\
        Y(j\omega)(j^2\omega^2 + 3j\omega + 2) &= X(j\omega) \\
        y''(t) + 3y'(t) + 2y(t) &= x(t) \\
    \end{align*}
    \item %write the solution of q3b
    \begin{align*}
        H(j\omega) &= H_1(j\omega)H_2(j\omega) \\
        H_1(j\omega) &= \frac{1}{j\omega + 1} \\
        H_2(j\omega) &= \frac{1}{j\omega + 2} \\
        H(j\omega) &= \frac{1}{j\omega + 1}\frac{1}{j\omega + 2} \\
        h_1(t) &= \mathcal{F}^{-1}\{H(j\omega)\} \\
        &= \mathcal{F}^{-1}\{\frac{1}{j\omega + 1}\frac{1}{j\omega + 2}\} \\
        &= \mathcal{F}^{-1}\{\frac{1}{j\omega + 1}\} * \mathcal{F}^{-1}\{\frac{1}{j\omega + 2}\} \\
        &= e^{-t}u(t) * e^{-2t}u(t) \\
        &= \int_{-\infty}^{\infty}e^{-(t - \tau)}u(t - \tau)e^{-2\tau}u(\tau)d\tau \\
        &= \int_{0}^{t}e^{-(t - \tau)}e^{-2\tau}d\tau \\
        &= \int_{0}^{t}e^{-t + \tau}e^{-2\tau}d\tau \\
        &= \int_{0}^{t}e^{-t}e^{\tau}e^{-2\tau}d\tau \\
        &= e^{-t}\int_{0}^{t}e^{-\tau}d\tau \\
        &= e^{-t}\left[-e^{-\tau}\right]_{0}^{t} \\
        &= e^{-t}\left[-e^{-t} + 1\right] \\
        &= e^{-t} - e^{-2t} \\
    \end{align*}
	\item %write the solution of q3c
    \begin{align*}
        X(j\omega) &= j\omega \\
        Y(j\omega) &= H(j\omega)X(j\omega) \\
        &= \frac{1}{j\omega + 1}\frac{1}{j\omega + 2}j\omega \\
        y(t) &= \mathcal{F}^{-1}\{Y(j\omega)\} \\
        &= \mathcal{F}^{-1}\{\frac{j\omega}{(j\omega + 1)(j\omega + 2)}\} \\
        &= \mathcal{F}^{-1}\{\frac{-1}{j\omega + 1} + \frac{2}{j\omega + 2}\} \\
        &= \mathcal{F}^{-1}\{\frac{-1}{j\omega + 1}\} + \mathcal{F}^{-1}\{\frac{2}{j\omega + 2}\} \\
        &= -e^{-t}u(t) + 2e^{-2t}u(t) \\
    \end{align*}
    \end{enumerate}

\item %write the solution of q4
    \begin{enumerate}   
    % Write your solutions in the following items.
    \item %write the solution of q4a
    \item %write the solution of q4b
	\item %write the solution of q4c
    \end{enumerate}

\item %write the solution of q5
        

\end{enumerate}


\end{document}

